done: local_sim -> gsim

src/ModAdequacy.v
@@ -12,9 +12,9 @@ Export ITreeNotations.
 From Fairness Require Import Axioms.
 From Fairness Require Export ITreeLib FairBeh FairSim NatStructs.
 From Fairness Require Import pind PCM World.
-From Fairness Require Export Mod ModSimGStutter Concurrency.
-From Fairness Require Import SchedSim Adequacy.
-From Fairness Require Import KnotSim LocalAdequacyAux Stutter2Knot Knot2Glob.
+From Fairness Require Export Mod Concurrency.
+From Fairness Require Import ModSimStutter KnotSim.
+From Fairness Require Import SchedSim Adequacy LocalAdequacyAux Stutter2Knot Knot2Glob.
 
 Set Implicit Arguments.
 
@@ -89,6 +89,115 @@ Section AUX.
     eapply IHFA; eauto. rewrite nm_find_rm_neq; auto. rewrite nm_find_rm_neq; auto. rewrite nm_find_rm_neq; auto.
   Qed.
 
+  Lemma nm_find_some_implies_forall3
+        elt1 elt2 elt3 (m1: NatMap.t elt1) (m2: NatMap.t elt2) (m3: NatMap.t elt3)
+        (P: elt1 -> elt2 -> elt3 -> key -> Prop)
+        (WFP1: nm_wf_pair m1 m2)
+        (WFP2: nm_wf_pair m1 m3)
+        (PROP: forall k e1 e2 e3
+                 (FIND1: find k m1 = Some e1) (FIND2: find k m2 = Some e2) (FIND3: find k m3 = Some e3), P e1 e2 e3 k)
+    :
+    Forall3 (fun '(k1, e1) '(k2, e2) '(k3, e3) => (k1 = k2) /\ (k1 = k3) /\ (P e1 e2 e3 k1))
+            (elements m1) (elements m2) (elements m3).
+  Proof.
+    remember (elements m1) as l1. move l1 before elt3. revert_until l1. induction l1; i; ss.
+    { symmetry in Heql1. apply elements_Empty in Heql1. dup Heql1.
+      hexploit nm_wf_pair_empty. eapply WFP1. i. apply H in Heql0. apply nm_empty_eq in Heql0. subst. rewrite elements_empty.
+      hexploit nm_wf_pair_empty. eapply WFP2. i. apply H0 in Heql1. apply nm_empty_eq in Heql1. subst. rewrite elements_empty.
+      econs.
+    }
+    destruct a as [k e1]. hexploit nm_elements_cons_rm. eauto. intros ELEM1. rewrite ELEM1 in Heql1.
+    destruct (elements m2) eqn:Heql2.
+    { exfalso. apply elements_Empty in Heql2. hexploit nm_wf_pair_empty. eapply WFP1. i. apply H in Heql2.
+      apply nm_empty_eq in Heql2. subst. rewrite elements_empty in Heql1. inv Heql1. }
+    destruct (elements m3) eqn:Heql3.
+    { exfalso. apply elements_Empty in Heql3. hexploit nm_wf_pair_empty. eapply WFP2. i. apply H in Heql3.
+      apply nm_empty_eq in Heql3. subst. rewrite elements_empty in Heql1. inv Heql1. }
+    destruct p as [k0 e2]. rename l into l2. symmetry in Heql2.
+    destruct p0 as [k1 e3]. rename l0 into l3. symmetry in Heql3.
+    hexploit nm_elements_cons_rm. eapply Heql2. intro ELEM2. rewrite ELEM2 in Heql2.
+    hexploit nm_elements_cons_rm. eapply Heql3. intro ELEM3. rewrite ELEM3 in Heql3.
+    assert (k = k0).
+    { hexploit nm_wf_pair_elements_forall2. eapply WFP1. rewrite <- Heql1, <- Heql2. i. inv H. auto. }
+    assert (k = k1).
+    { hexploit nm_wf_pair_elements_forall2. eapply WFP2. rewrite <- Heql1, <- Heql3. i. inv H0. auto. }
+    replace k0 with k in *. replace k1 with k in *. clear H H0. econs.
+    2:{ rewrite ELEM2, ELEM3. eapply IHl1; eauto.
+        apply nm_wf_pair_rm; auto. apply nm_wf_pair_rm; auto.
+        i. eapply PROP.
+        rewrite F.remove_o in FIND1. des_ifs. rewrite F.remove_o in FIND2. des_ifs. rewrite F.remove_o in FIND3. des_ifs.
+    }
+    splits; auto. eapply PROP. all: eapply nm_elements_cons_find_some; eauto.
+  Qed.
+
+  Inductive Forall4 (A B C D : Type) (R : A -> B -> C -> D -> Prop) : list A -> list B -> list C -> list D -> Prop :=
+    Forall4_nil : Forall4 R [] [] [] []
+  | Forall4_cons : forall (x : A) (y : B) (z : C) (w : D) (l1 : list A) (l2 : list B) (l3: list C) (l4: list D),
+      R x y z w -> Forall4 R l1 l2 l3 l4 -> Forall4 R (x :: l1) (y :: l2) (z :: l3) (w :: l4).
+
+  Lemma list_forall4_implies_forall2_4
+        A B C D (f1: A -> B -> C -> D -> Prop) (f2: A -> D -> Prop)
+        la lb lc ld
+        (FA: Forall4 f1 la lb lc ld)
+        (IMP: forall a b c d, (f1 a b c d) -> (f2 a d))
+    :
+    List.Forall2 f2 la ld.
+  Proof.
+    move FA before D. revert_until FA. induction FA; i; ss. econs; eauto.
+  Qed.
+
+  Lemma list_forall4_implies_forall2_3
+        A B C D (f1: A -> B -> C -> D -> Prop) (f2: A -> C -> Prop)
+        la lb lc ld
+        (FA: Forall4 f1 la lb lc ld)
+        (IMP: forall a b c d, (f1 a b c d) -> (f2 a c))
+    :
+    List.Forall2 f2 la lc.
+  Proof.
+    move FA before D. revert_until FA. induction FA; i; ss. econs; eauto.
+  Qed.
+
+  Lemma list_forall4_implies_forall2_2
+        A B C D (f1: A -> B -> C -> D -> Prop) (f2: A -> B -> Prop)
+        la lb lc ld
+        (FA: Forall4 f1 la lb lc ld)
+        (IMP: forall a b c d, (f1 a b c d) -> (f2 a b))
+    :
+    List.Forall2 f2 la lb.
+  Proof.
+    move FA before D. revert_until FA. induction FA; i; ss. econs; eauto.
+  Qed.
+
+  Import NatMap.
+  Import NatMapP.
+
+  Lemma nm_forall4_implies_find_some
+        elt1 elt2 elt3 elt4 (m1: NatMap.t elt1) (m2: NatMap.t elt2) (m3: NatMap.t elt3) (m4: NatMap.t elt4)
+        P
+        (FA: Forall4 (fun '(k1, e1) '(k2, e2) '(k3, e3) '(k4, e4) => (k1 = k2) /\ (k1 = k3) /\ (k1 = k4) /\ (P e1 e2 e3 e4 k1))
+                     (elements m1) (elements m2) (elements m3) (elements m4))
+    :
+    forall k e1 e2 e3 e4
+      (FIND1: find k m1 = Some e1) (FIND2: find k m2 = Some e2) (FIND3: find k m3 = Some e3) (FIND4: find k m4 = Some e4),
+      P e1 e2 e3 e4 k.
+  Proof.
+    match goal with
+    | FA: Forall4 _ ?_ml1 ?_ml2 ?_ml3 ?_ml4 |- _ =>
+        remember _ml1 as ml1; remember _ml2 as ml2; remember _ml3 as ml3; remember _ml4 as ml4
+    end.
+    move FA before elt4. revert_until FA. induction FA; i.
+    { symmetry in Heqml1; apply elements_Empty in Heqml1.
+      apply nm_empty_eq in Heqml1. subst. rewrite F.empty_o in FIND1; ss.
+    }
+    des_ifs. des; clarify. destruct (F.eq_dec k k3); clarify.
+    { eapply nm_elements_cons_find_some in Heqml1, Heqml2, Heqml3, Heqml4. clarify. }
+    hexploit nm_elements_cons_rm. eapply Heqml1. intro RM1.
+    hexploit nm_elements_cons_rm. eapply Heqml2. intro RM2.
+    hexploit nm_elements_cons_rm. eapply Heqml3. intro RM3.
+    hexploit nm_elements_cons_rm. eapply Heqml4. intro RM4.
+    eapply IHFA; eauto. all: rewrite nm_find_rm_neq; auto.
+  Qed.
+
 End AUX.
 
 
@@ -111,9 +220,10 @@ Section LADEQ.
   Notation srcE := ((@eventE _ident_src +' cE) +' sE state_src).
   Notation tgtE := ((@eventE _ident_tgt +' cE) +' sE state_tgt).
 
-  Variable wf_stt: WF.
+  Variable wf_stt: Type -> Type -> WF.
+  Let nm_wf_stt: Type -> Type -> WF := nm_wf_stt wf_stt.
 
-  Let shared := shared state_src state_tgt _ident_src _ident_tgt wf_src wf_tgt wf_stt.
+  Let shared := shared state_src state_tgt _ident_src _ident_tgt wf_src wf_tgt.
 
   Notation threads_src1 R0 := (threads _ident_src (sE state_src) R0).
   Notation threads_src2 R0 := (threads2 _ident_src (sE state_src) R0).
@@ -135,22 +245,40 @@ Section LADEQ.
         src tgt
         (st_src: state_src) (st_tgt: state_tgt)
         ps pt
-        (LSIM: forall im_tgt, exists im_src o r_shared rs_ctx,
+        (LSIM: forall im_tgt, exists im_src r_shared (os: (nm_wf_stt R0 R1).(T)) rs_ctx o,
             (<<RSWF: Th.find tid rs_ctx = None>>) /\
+              (<<OSWF: (forall tid', Th.In tid' ths_src -> Th.In tid' os) /\ (Th.find tid os = None)>>) /\
               (<<LSIM:
                 forall im_tgt0
                   (FAIR: fair_update im_tgt im_tgt0 (sum_fmap_l (tids_fmap tid (NatSet.add tid (key_set ths_tgt))))),
                 exists im_src0,
                   (fair_update im_src im_src0 (sum_fmap_l (tids_fmap tid (NatSet.add tid (key_set ths_src))))) /\
-                    (lsim I (local_RR I RR tid) tid ps pt (sum_of_resources rs_ctx)
-                          src tgt
-                          (NatSet.add tid (key_set ths_src), NatSet.add tid (key_set ths_tgt),
-                            im_src0, im_tgt0, st_src, st_tgt, o, r_shared))>>) /\
-              (<<LOCAL: forall tid (src: itree srcE R0) (tgt: itree tgtE R1) r_own
+                    (lsim (wf_stt) I tid (local_RR I RR tid)
+                          ps pt (sum_of_resources rs_ctx) (o, src) tgt
+                          (NatSet.add tid (key_set ths_src),
+                            im_src0, im_tgt0, st_src, st_tgt, r_shared))>>) /\
+              (<<LOCAL: forall tid (src: itree srcE R0) (tgt: itree tgtE R1) o r_own
                           (OWN: r_own = fst (get_resource tid rs_ctx))
                           (LSRC: Th.find tid ths_src = Some src)
-                          (LTGT: Th.find tid ths_tgt = Some tgt),
-                  (local_sim_pick I RR src tgt tid r_own)>>))
+                          (LTGT: Th.find tid ths_tgt = Some tgt)
+                          (ORD: Th.find tid os = Some o),
+                    (local_sim_pick wf_stt I RR src tgt tid o r_own)>>))
+        (* (LSIM: forall im_tgt, exists im_src o r_shared rs_ctx, *)
+        (*     (<<RSWF: Th.find tid rs_ctx = None>>) /\ *)
+        (*       (<<LSIM: *)
+        (*         forall im_tgt0 *)
+        (*           (FAIR: fair_update im_tgt im_tgt0 (sum_fmap_l (tids_fmap tid (NatSet.add tid (key_set ths_tgt))))), *)
+        (*         exists im_src0, *)
+        (*           (fair_update im_src im_src0 (sum_fmap_l (tids_fmap tid (NatSet.add tid (key_set ths_src))))) /\ *)
+        (*             (lsim I (local_RR I RR tid) tid ps pt (sum_of_resources rs_ctx) *)
+        (*                   src tgt *)
+        (*                   (NatSet.add tid (key_set ths_src), NatSet.add tid (key_set ths_tgt), *)
+        (*                     im_src0, im_tgt0, st_src, st_tgt, o, r_shared))>>) /\ *)
+        (*       (<<LOCAL: forall tid (src: itree srcE R0) (tgt: itree tgtE R1) r_own *)
+        (*                   (OWN: r_own = fst (get_resource tid rs_ctx)) *)
+        (*                   (LSRC: Th.find tid ths_src = Some src) *)
+        (*                   (LTGT: Th.find tid ths_tgt = Some tgt), *)
+        (*           (local_sim_pick I RR src tgt tid r_own)>>)) *)
     :
     gsim wf_src wf_tgt RR
          (interp_all st_src (Th.add tid src ths_src) tid)
@@ -169,6 +297,7 @@ Section LADEQ.
     replace (NatSet.add tid (key_set ths_src2)) with (NatSet.add tid (key_set ths_src)).
     2:{ unfold key_set. clarify. rewrite nm_map_unit1_map_eq. auto. }
     esplits; eauto.
+    { i. apply OSWF. rewrite Heqths_src2 in H. eapply Th.map_2 in H. auto. }
     i. assert (SF: sf = false).
     { clarify. rewrite NatMapP.F.map_o in LSRC.
       destruct (NatMap.find (elt:=thread _ident_src (sE state_src) R0) tid0 ths_src); ss. clarify. }
@@ -184,7 +313,7 @@ Section LADEQ.
              (ths_tgt: threads_tgt R1)
     :=
     List.Forall2
-      (fun '(t1, src) '(t2, tgt) => (t1 = t2) /\ (local_sim I RR src tgt))
+      (fun '(t1, src) '(t2, tgt) => (t1 = t2) /\ (local_sim wf_stt I RR src tgt))
       (Th.elements ths_src) (Th.elements ths_tgt).
 
   Lemma local_sim_threads_local_sim_pick
@@ -193,19 +322,18 @@ Section LADEQ.
         (ths_tgt: threads_tgt R1)
         (LOCAL: local_sim_threads RR ths_src ths_tgt)
         (st_src: state_src) (st_tgt: state_tgt)
-        (INV: forall im_tgt, exists im_src o r_shared,
-            (I (NatSet.empty, NatSet.empty, im_src, im_tgt, st_src, st_tgt, o, r_shared)) /\
-              (URA.wf r_shared))
+        (INV: forall im_tgt, exists im_src r_shared,
+            (I (NatSet.empty, im_src, im_tgt, st_src, st_tgt, r_shared)) /\ (URA.wf r_shared))
     :
     forall im_tgt,
-    exists (im_src0 : imap ident_src wf_src) (o0 : T wf_stt) r_shared0 (rs_local: local_resources),
-      (I (key_set ths_src, key_set ths_tgt, im_src0, im_tgt, st_src, st_tgt, o0, r_shared0)) /\
+    exists (im_src0 : imap ident_src wf_src) r_shared0 (os: (nm_wf_stt R0 R1).(T)) (rs_local: local_resources),
+      (I (key_set ths_src, im_src0, im_tgt, st_src, st_tgt, r_shared0)) /\
         (resources_wf r_shared0 rs_local) /\
-        (Forall3 (fun '(t1, src) '(t2, tgt) '(t3, r_own) =>
-                    (t1 = t2) /\ (t1 = t3) /\ (local_sim_pick I RR src tgt t1 r_own))
+        (Forall4 (fun '(t1, src) '(t2, tgt) '(t3, r_own) '(t4, o) =>
+                    (t1 = t2) /\ (t1 = t3) /\ (t1 = t4) /\ (local_sim_pick wf_stt I RR src tgt t1 o r_own))
                  (Th.elements (elt:=thread _ident_src (sE state_src) R0) ths_src)
                  (Th.elements (elt:=thread _ident_tgt (sE state_tgt) R1) ths_tgt)
-                 (Th.elements rs_local)).
+                 (Th.elements rs_local) (Th.elements os)).
   Proof.
     unfold local_sim_threads in LOCAL.
     match goal with
@@ -219,7 +347,7 @@ Section LADEQ.
       esplits; ss; eauto.
       - unfold NatSet.empty in *. rewrite !key_set_empty_empty_eq. eauto.
       - instantiate (1:=@NatMap.empty _). unfold resources_wf. r_wf INV0. rewrite sum_of_resources_empty. r_solve.
-      - econs.
+      - instantiate (1:=NatMap.empty _). econs.
     }
 
     des_ifs. des; clarify. rename k0 into tid1, i into src1, i0 into tgt1.
@@ -228,30 +356,46 @@ Section LADEQ.
     hexploit IHLOCAL; clear IHLOCAL; eauto. intro IND.
     des. clear INV.
     unfold local_sim in H0.
-    specialize (H0 _ _ _ _ _ _ _ _ (sum_of_resources rs_local) IND tid1 (key_set ths_src) (key_set ths_tgt)).
+    specialize (H0 _ _ _ _ _ _ (sum_of_resources rs_local) IND tid1 (key_set ths_src)).
     hexploit H0; clear H0.
     { econs. rewrite key_set_pull_rm_eq. eapply nm_find_rm_eq.
       erewrite <- key_set_pull_add_eq. instantiate (1:=src1).
       rewrite <- nm_find_some_rm_add_eq; auto. eapply nm_elements_cons_find_some; eauto.
     }
-    { econs. rewrite key_set_pull_rm_eq. eapply nm_find_rm_eq.
-      erewrite <- key_set_pull_add_eq. instantiate (1:=tgt1).
-      rewrite <- nm_find_some_rm_add_eq; auto. eapply nm_elements_cons_find_some; eauto.
-    }
     { r_wf IND0. }
     instantiate (1:=im_tgt). i; des.
     assert (WFPAIR: nm_wf_pair (NatMap.remove (elt:=thread _ident_src (sE state_src) R0) tid1 ths_src) rs_local).
-    { hexploit list_forall3_implies_forall2_3. eauto.
+    { hexploit list_forall4_implies_forall2_3. eauto.
       { i. instantiate (1:=fun '(t1, src) '(t3, r_own) => t1 = t3). ss. des_ifs. des; auto. }
       intros FA2. rewrite RESS in FA2. apply nm_forall2_wf_pair in FA2. auto.
     }
     assert (RSL: NatMap.find (elt:=M) tid1 rs_local = None).
     { eapply nm_wf_pair_find_cases in WFPAIR. des. eapply WFPAIR. apply nm_find_rm_eq. }
+    assert (WFPAIRO: nm_wf_pair (NatMap.remove (elt:=thread _ident_src (sE state_src) R0) tid1 ths_src) os).
+    { hexploit list_forall4_implies_forall2_4. eauto.
+      { i. instantiate (1:=fun '(t1, src) '(t4, o) => t1 = t4). ss. des_ifs. des; auto. }
+      intros FA2. rewrite RESS in FA2. apply nm_forall2_wf_pair in FA2. auto.
+    }
+    assert (FINDOS: NatMap.find tid1 os = None).
+    { eapply nm_wf_pair_find_cases in WFPAIRO. des. eapply WFPAIRO. apply nm_find_rm_eq. }
+
     esplits; eauto.
     { instantiate (1:=Th.add tid1 r_own rs_local). unfold resources_wf. rewrite sum_of_resources_add. r_wf VALID. auto. }
     replace (Th.elements (Th.add tid1 r_own rs_local)) with ((tid1, r_own) :: (Th.elements rs_local)).
-    { econs; auto. splits; ss. ii.
-      specialize (H1 _ _ _ _ _ _ _ _ _ INV0 VALID0 im_tgt1 FAIR). des. esplits; eauto.
+    instantiate (1:=Th.add tid1 o os).
+    replace (Th.elements (Th.add tid1 o os)) with ((tid1, o) :: (Th.elements os)).
+    { econs; auto. }
+    { remember (Th.add tid1 o os) as os1.
+      assert (REP: os = (NatMap.remove tid1 os1)).
+      { rewrite Heqos1. rewrite nm_find_none_rm_add_eq; auto. }
+      rewrite REP. rewrite REP in WFPAIRO. rewrite RESS in Heqtl_src.
+      eapply wf_pair_elements_cons_rm; eauto.
+      { eapply nm_wf_pair_rm_inv; eauto.
+        - unfold NatMap.In, NatMap.Raw.PX.In. exists src1. unfold NatMap.Raw.PX.MapsTo. ss.
+          unfold Th.elements, Th.Raw.elements in Heqtl_src. rewrite <- Heqtl_src. econs 1. ss.
+        - rewrite Heqos1. apply NatMapP.F.add_in_iff. auto.
+      }
+      { rewrite Heqos1. rewrite nm_find_add_eq; auto. }
     }
     { remember (Th.add tid1 r_own rs_local) as rs_local1.
       assert (REP: rs_local = (NatMap.remove tid1 rs_local1)).
@@ -273,9 +417,8 @@ Section LADEQ.
           (ths_tgt: threads_tgt R1)
           (LOCAL: local_sim_threads RR ths_src ths_tgt)
           (st_src: state_src) (st_tgt: state_tgt)
-          (INV: forall im_tgt, exists im_src o r_shared,
-              (I (NatSet.empty, NatSet.empty, im_src, im_tgt, st_src, st_tgt, o, r_shared)) /\
-                (URA.wf r_shared))
+          (INV: forall im_tgt, exists im_src r_shared,
+              (I (NatSet.empty, im_src, im_tgt, st_src, st_tgt, r_shared)) /\ (URA.wf r_shared))
           tid
           (INS: Th.In tid ths_src)
           (INT: Th.In tid ths_tgt)
@@ -302,72 +445,91 @@ Section LADEQ.
     replace ths_tgt with (Th.add tid tgt0 ths_tgt0).
     2:{ symmetry; eapply nm_pop_res_is_add_eq; eauto. }
 
-    eapply lsim_implies_gsim; auto.
+    assert (WFST0: nm_wf_pair ths_src0 ths_tgt0).
     { subst. eapply nm_wf_pair_rm. eapply nm_forall2_wf_pair.
       eapply list_forall2_implies; eauto. i. des_ifs. des; auto.
     }
+    eapply lsim_implies_gsim; auto.
     { eapply nm_pop_res_find_none; eauto. }
     { eapply nm_pop_res_find_none; eauto. }
 
-    cut (forall im_tgt0, exists im_src0 o0 r_shared0 rs_ctx0,
-            (I (key_set ths_src, key_set ths_tgt, im_src0, im_tgt0, st_src, st_tgt, o0, r_shared0)) /\
+    cut (forall im_tgt0, exists im_src0 r_shared0 (os0: (nm_wf_stt R0 R1).(T)) rs_ctx0,
+            (I (key_set ths_src, im_src0, im_tgt0, st_src, st_tgt, r_shared0)) /\
               (resources_wf r_shared0 rs_ctx0) /\
+              (nm_wf_pair ths_src os0) /\
               (forall (tid0 : Th.key) (src : thread _ident_src (sE state_src) R0)
-                 (tgt : thread _ident_tgt (sE state_tgt) R1) r_own,
+                 (tgt : thread _ident_tgt (sE state_tgt) R1) o r_own,
                   (r_own = fst (get_resource tid0 rs_ctx0)) ->
                   (Th.find (elt:=thread _ident_src (sE state_src) R0) tid0 ths_src = Some src) ->
                   (Th.find (elt:=thread _ident_tgt (sE state_tgt) R1) tid0 ths_tgt = Some tgt) ->
-                  local_sim_pick I RR src tgt tid0 r_own)).
-    { i. specialize (H im_tgt). des. exists im_src0, o0, r_shared0, (snd (get_resource tid rs_ctx0)). splits.
+                  (Th.find tid0 os0 = Some o) ->
+                  local_sim_pick wf_stt I RR src tgt tid0 o r_own)).
+    { i. specialize (H im_tgt). des.
+      assert (POPOS: exists o os, nm_pop tid os0 = Some (o, os)).
+      { hexploit nm_wf_pair_pop_cases. eapply H1. instantiate (1:=tid). i; des; eauto.
+        unfold nm_pop in H3. rewrite FINDS in H3. ss. }
+      des. exists im_src0, r_shared0, os, (snd (get_resource tid rs_ctx0)), o. splits.
       - eapply get_resource_snd_find_eq_none.
-      - ii. specialize (H1 tid src0 tgt0 (fst (get_resource tid rs_ctx0))). hexploit H1; clear H1; auto.
-        i. unfold local_sim_pick in H1.
+      - i. eapply nm_wf_pair_pop_cases in H1. des. erewrite POPS in H1. ss.
+        rewrite POPS in H1; rewrite POPOS in H4. clarify.
+        eapply nm_wf_pair_find_cases in H5. des. eapply NatMapP.F.in_find_iff. eapply H1.
+        eapply NatMapP.F.in_find_iff. auto.
+      - eapply find_none_aux; eauto.
+      - ii. specialize (H2 tid src0 tgt0 o (fst (get_resource tid rs_ctx0))). hexploit H2; clear H2; auto.
+        { eapply nm_pop_find_some; eauto. }
+        i. unfold local_sim_pick in H2.
         assert (SETS: NatSet.add tid (key_set ths_src0) = key_set ths_src).
         { subst. rewrite key_set_pull_rm_eq. unfold NatSet.add.
           rewrite <- nm_find_some_rm_add_eq; auto. eapply key_set_find_some1; eauto.
         }
-        assert (SETT: NatSet.add tid (key_set ths_tgt0) = key_set ths_tgt).
-        { subst. rewrite key_set_pull_rm_eq. unfold NatSet.add.
-          rewrite <- nm_find_some_rm_add_eq; auto. eapply key_set_find_some1; eauto.
-        }
-        hexploit H1; clear H1. eapply H.
+        hexploit H2; clear H2. eapply H.
         { instantiate (1:=sum_of_resources (snd (get_resource tid rs_ctx0))).
           hexploit resources_wf_get_wf. eapply H0.
           2:{ i. des. eapply WF. }
           instantiate (1:=tid). destruct (get_resource tid rs_ctx0); ss.
         }
-        { rewrite <- SETT; eauto. }
-        rewrite !SETS, !SETT. eauto.
-      - i. eapply H1.
+        { rewrite <- SETS; eauto. unfold nm_wf_pair in WFST0. rewrite WFST0. eauto. }
+        rewrite !SETS. i; des. esplits; eauto.
+      - i. eapply H2.
         { rewrite OWN. eapply get_resource_rs_neq. destruct (tid_dec tid tid0); auto. clarify.
           rewrite nm_find_rm_eq in LSRC. ss. }
-        eapply find_some_aux; eauto. eapply find_some_aux; eauto.
+        eapply find_some_aux; eauto. eapply find_some_aux; eauto. eapply find_some_aux; eauto.
     }
 
-    cut (forall im_tgt, exists (im_src0 : imap ident_src wf_src) (o0 : T wf_stt) r_shared0 rs_ctx0,
-            I (key_set ths_src, key_set ths_tgt, im_src0, im_tgt, st_src, st_tgt, o0, r_shared0) /\
+    cut (forall im_tgt, exists (im_src0 : imap ident_src wf_src) r_shared0 (os0: (nm_wf_stt R0 R1).(T)) rs_ctx0,
+            I (key_set ths_src, im_src0, im_tgt, st_src, st_tgt, r_shared0) /\
               (resources_wf r_shared0 rs_ctx0) /\
-              (List.Forall2 (fun '(t1, src) '(t2, tgt) =>
-                               (t1 = t2) /\ local_sim_pick I RR src tgt t1 (fst (get_resource t1 rs_ctx0)))
-                            (Th.elements (elt:=thread _ident_src (sE state_src) R0) ths_src)
-                            (Th.elements (elt:=thread _ident_tgt (sE state_tgt) R1) ths_tgt))).
-    { intro FA. i. specialize (FA im_tgt0). des. esplits; eauto. i. subst.
-      eapply nm_forall2_implies_find_some in FA1; eauto.
+              (Forall3 (fun '(t1, src) '(t2, tgt) '(t3, o) =>
+                          (t1 = t2) /\ (t1 = t3) /\
+                            (local_sim_pick wf_stt I RR src tgt t1 o (fst (get_resource t1 rs_ctx0))))
+                       (Th.elements (elt:=thread _ident_src (sE state_src) R0) ths_src)
+                       (Th.elements (elt:=thread _ident_tgt (sE state_tgt) R1) ths_tgt)
+                       (Th.elements os0))).
+    { intro FA. i. specialize (FA im_tgt0). des. esplits; eauto.
+      { hexploit list_forall3_implies_forall2_3. eauto.
+        { i. instantiate (1:= fun '(t1, src) '(t3, o) => t1 = t3). ss. des_ifs. des; auto. }
+        intros FA2. apply nm_forall2_wf_pair in FA2. eauto.
+      }
+      i. subst. eapply nm_forall3_implies_find_some in FA1; eauto.
     }
 
     i. hexploit local_sim_threads_local_sim_pick; eauto. intros FAALL. instantiate (1:=im_tgt) in FAALL.
     clear LOCAL. des.
-    exists im_src0, o0, r_shared0, rs_local. splits; auto.
+    exists im_src0, r_shared0, os, rs_local. splits; auto.
     clear - FAALL1.
-    eapply nm_find_some_implies_forall2.
-    { hexploit list_forall3_implies_forall2_2. eauto.
+    eapply nm_find_some_implies_forall3.
+    { hexploit list_forall4_implies_forall2_2. eauto.
       { i. instantiate (1:=fun '(t1, src) '(t2, tgt) => t1 = t2). ss. des_ifs. des; auto. }
       intros FA2. apply nm_forall2_wf_pair; auto.
     }
-    { i. hexploit nm_forall3_implies_find_some. eapply FAALL1. all: eauto.
+    { hexploit list_forall4_implies_forall2_4. eauto.
+      { i. instantiate (1:=fun '(t1, src) '(t4, o) => t1 = t4). ss. des_ifs. des; auto. }
+      intros FA2. apply nm_forall2_wf_pair; auto.
+    }
+    { i. hexploit nm_forall4_implies_find_some. eapply FAALL1. all: eauto.
       2:{ ss. eauto. }
       assert (WFPAIR: nm_wf_pair ths_src rs_local).
-      { hexploit list_forall3_implies_forall2_3. eauto.
+      { hexploit list_forall4_implies_forall2_3. eauto.
         { i. instantiate (1:=fun '(t1, src) '(t3, r_own) => t1 = t3). ss. des_ifs. des; auto. }
         intros FA2. apply nm_forall2_wf_pair in FA2. auto.
       }
