src/Knot2Glob.v
@@ -12,7 +12,7 @@ Export ITreeNotations.
 From Fairness Require Import Axioms.
 From Fairness Require Export ITreeLib FairBeh FairSim NatStructs.
 From Fairness Require Import pind PCM World.
-From Fairness Require Export Mod ModSimGStutter Concurrency.
+From Fairness Require Export Mod Concurrency.
 From Fairness Require Import KnotSim LocalAdequacyAux.
 
 Set Implicit Arguments.
